adequacy for a small pl

theories/semtype.v
@@ -1,18 +1,18 @@
 From stdpp Require Import base.
 From iris.base_logic Require Import upred.
 From iris.base_logic.lib Require Import iprop own.
+From iris.bi Require Import updates.
 From iris.algebra Require Import ofe cmra gmap_view.
 From iris.proofmode Require Import tactics.
 
 Definition tag := positive.
-Definition loc := positive.
-Inductive value : Set :=
-  | UnitV
-  | LocV (ℓ : loc).
-Canonical Structure valueO : ofe := leibnizO value.
-Local Instance value_inhabited : Inhabited value := populate UnitV.
-
 Canonical Structure tagO : ofe := discreteO tag.
+
+Definition loc := positive.
+
+Inductive value : Set :=
+  | IntV (n : Z)
+  | LocV (ℓ : loc).
 
 (* interpretation of types *)
 Definition sem_typeO (Σ : gFunctors) : ofe := value -d> iPropO Σ.
@@ -22,7 +22,7 @@ Class sem_heapG (Σ : gFunctors) : Set := SemHeapG {
 }.
 
 Inductive lang_ty := 
-  | UnitT
+  | IntT
   | UnionT (A : lang_ty) (B : lang_ty)
   | ClassT (t : tag).
 Canonical Structure lang_tyO : ofe := leibnizO lang_ty.
@@ -46,8 +46,8 @@ Eval hnf in interp.
 
 (* now, let's interpret some types *)
 
-Definition interp_unit : interp :=
-  λ (v : value), ⌜v = UnitV⌝%I.
+Definition interp_int : interp :=
+  λ (v : value), ⌜∃ n, v = IntV n⌝%I.
 
 Definition interp_union (iA : interp) (iB : interp) : interp :=
   λ (w : value), (iA w ∨ iB w)%I.
@@ -75,7 +75,7 @@ Definition interp_type_pre (rec : ty_interpO) : ty_interpO :=
   λ (ty : lang_ty),
     (fix go (ty : lang_ty) : interp :=
        match ty with
-       | UnitT => interp_unit
+       | IntT => interp_int
        | UnionT A B => interp_union (go A) (go B)
        | ClassT t => interp_class t rec
        end) ty.
@@ -106,11 +106,24 @@ Global Instance interp_type_persistent (ty : lang_ty) (v : value) :
 Proof.
   elim: ty => [].
   - rewrite interp_type_unfold. apply _.
-  - move=> A Ha B Hb. rewrite interp_type_unfold /=.
+  - move=>>. rewrite interp_type_unfold /=.
     rewrite /interp_union. rewrite -!interp_type_unfold.
     by apply bi.or_persistent.
-  - move=>?. rewrite interp_type_unfold /=.
-    rewrite /interp_class. apply _.
+  - move=>>. rewrite interp_type_unfold. apply _.
+Qed.
+
+(* that is a bit of an awkward lemma;
+   I am not yet sure it "scales" *)
+Lemma interp_type_loc_inversion ty ℓ :
+  interp_type ty (LocV ℓ) -∗
+  ∃ t, interp_type (ClassT t) (LocV ℓ).
+Proof.
+  rewrite interp_type_unfold. elim: ty => /=.
+  - iIntros "%". naive_solver.
+  - move=>? IH1 ? IH2. iIntros "[H|H]".
+    by iApply IH1. by iApply IH2.
+  - move=> t. iIntros "H". iExists t.
+    by rewrite interp_type_unfold /=.
 Qed.
 
 (* concrete heaps *)
@@ -128,8 +141,8 @@ Definition heap_models (h : heap) : iProp :=
 Example alloc_unit_class_lemma (h : heap) (new : loc) (t : tag) :
   h !! new = None →
   heap_models h -∗ |==>
-  heap_models (<[ new := (t, UnitV) ]> h) ∗
-  sem_heap_mapsto new t (interp_type UnitT).
+  heap_models (<[ new := (t, IntV 0) ]> h) ∗
+  sem_heap_mapsto new t (interp_type IntT).
 Proof.
   move=> Hnew. iIntros "Hm". iDestruct "Hm" as (sh) "[Hown [Hdom #Hm]]".
   iDestruct "Hdom" as %Hdom.
@@ -147,7 +160,7 @@ Proof.
   - iExists _. rewrite lookup_insert.
     iSplitR; first done.
     rewrite interp_type_unfold /=.
-    by rewrite /interp_unit.
+    rewrite /interp_int. by eauto.
   - iDestruct ("Hm" with "[]") as (iF) "[Heq HiF]"; first done.
     case Hsh : (sh !! ℓ) => [[]|].
     + iExists _. iSplitR "HiF"; last done.
@@ -243,6 +256,459 @@ Proof.
   - iDestruct ("Hm" $! l' with "[//]") as (iF) "[??]".
     iExists _. rewrite lookup_insert_ne; last done.
     iSplit; eauto.
+Qed.
+
+(* language statics & semantics *)
+
+Definition var := positive.
+
+Inductive lang_expr : Type :=
+  | VarE (v : var)
+  | LitE (lit : Z)
+  | OpE (op : Z → Z → Z)
+        (lhs rhs : lang_expr).
+
+Inductive lang_cmd : Type :=
+  | LetC (v : var) (e : lang_expr)  (* local def *)
+  | NewC (v : var) (t : tag)        (* allocation *)
+  | GetC (v : var) (e : lang_expr)  (* field read *)
+  | SetC (lhs rhs : lang_expr)      (* fiels store *)
+  | SeqC (fstc sndc : lang_cmd)     (* sequence *)
+  | CondC (cnd : lang_expr)
+          (ifc elc : lang_cmd)      (* conditional *)
+  | CondTagC (v : var) (t : tag)
+             (cmd : lang_cmd)       (* tag test
+                                       "if ($v is C) { ... }" *)
+  | WhileC (cnd : lang_expr)
+           (cmd : lang_cmd)         (* while loop *).
+
+(* programs are a command and a 'return'
+   expression *)
+Record lang_prog : Type :=
+  Prog { prog_body : lang_cmd;
+         prog_ret : lang_expr }.
+
+Definition local_tys := gmap var lang_ty.
+
+Inductive expr_has_ty (lty : local_tys) :
+    lang_expr → lang_ty → Prop :=
+  | VarTy (v : var) (ty : lang_ty) :
+      lty !! v = Some ty →
+      expr_has_ty lty (VarE v) ty
+  | LitTy (lit : Z) :
+      expr_has_ty lty (LitE lit) IntT
+  | OpTy (op : Z → Z → Z) (lhs rhs : lang_expr) :
+      expr_has_ty lty lhs IntT →
+      expr_has_ty lty rhs IntT →
+      expr_has_ty lty (OpE op lhs rhs) IntT.
+
+(* continuation-based typing for commands *)
+Inductive cmd_has_ty :
+    local_tys → lang_cmd → local_tys → Prop :=
+  | LetTy lty v e ty :
+      expr_has_ty lty e ty →
+      cmd_has_ty lty (LetC v e) (<[v:=ty]> lty)
+  | NewTy lty v t :
+      cmd_has_ty lty (NewC v t) (<[v:=ClassT t]> lty)
+  | GetTy lty v e t ty :
+      Δ !! t = Some ty →
+      expr_has_ty lty e (ClassT t) →
+      cmd_has_ty lty (GetC v e) (<[v:=ty]> lty)
+  | SetTy lty lhs rhs t ty :
+      Δ !! t = Some ty →
+      expr_has_ty lty lhs (ClassT t) →
+      expr_has_ty lty rhs ty →
+      cmd_has_ty lty (SetC lhs rhs) lty
+  | SeqTy lty1 lty2 lty3 fstc sndc :
+      cmd_has_ty lty1 fstc lty2 →
+      cmd_has_ty lty2 sndc lty3 →
+      cmd_has_ty lty1 (SeqC fstc sndc) lty3
+  | CondTy lty1 lty2 cnd ifc elc :
+      expr_has_ty lty1 cnd IntT →
+      cmd_has_ty lty1 ifc lty2 →
+      cmd_has_ty lty1 elc lty2 →
+      cmd_has_ty lty1 (CondC cnd ifc elc) lty2
+  | CondTagTy lty v t cmd :
+      (* we do not care about v's type but it's
+         got to have one! (i.e., be defined) *)
+      is_Some (lty !! v) →
+      cmd_has_ty (<[v:=ClassT t]> lty) cmd lty →
+      cmd_has_ty lty (CondTagC v t cmd) lty
+  | WhileTy lty cnd cmd :
+      expr_has_ty lty cnd IntT →
+      cmd_has_ty lty cmd lty →
+      cmd_has_ty lty (WhileC cnd cmd) lty.
+
+Inductive prog_has_ty : lang_prog → lang_ty → Prop :=
+  | ProgTy lty ty body ret :
+      cmd_has_ty ∅ body lty →
+      expr_has_ty lty ret ty →
+      prog_has_ty (Prog body ret) ty.
+
+Definition local_env := gmap var value.
+
+Inductive expr_eval (le : local_env) :
+    lang_expr → value → Prop :=
+  | VarEv v val :
+      le !! v = Some val →
+      expr_eval le (VarE v) val
+  | LitEv lit :
+      expr_eval le (LitE lit) (IntV lit)
+  | OpEv op lhs rhs nl nr :
+      expr_eval le lhs (IntV nl) →
+      expr_eval le rhs (IntV nr) →
+      expr_eval le (OpE op lhs rhs) (IntV (op nl nr)).
+
+Definition value_trueish := λ v,
+  match v with
+  | IntV n => n <> 0
+  | _ => True
+  end.
+
+Global Instance value_trueish_decision (v : value) :
+  Decision (value_trueish v).
+Proof. move: v => []; apply _. Defined.
+
+Definition tag_match (st : local_env * heap) v t :=
+  ∃ l, st.1 !! v = Some (LocV l) ∧
+       ∃ v, st.2 !! l = Some (t, v).
+
+Global Instance tag_match_decision st v t:
+    Decision (tag_match st v t).
+Proof.
+  move: st => [le h]. rewrite /tag_match /=.
+  move: (le !! v) => [[]|];
+    try (right; naive_solver).
+  move=> l. case_eq (h !! l);
+    last (right; naive_solver).
+  move=> [t' ?] ?.
+  destruct (decide (t = t')) as [->|];
+    last (right; naive_solver).
+  left. eauto.
+Defined.
+
+Inductive cmd_eval :
+    (local_env * heap) → lang_cmd →
+    (local_env * heap) → Prop :=
+  | LetEv le h v e ve :
+      expr_eval le e ve →
+      cmd_eval (le, h) (LetC v e) (<[v:=ve]> le, h)
+  | NewEv le h l v t :
+      h !! l = None →
+      Δ !! t = Some IntT →
+      cmd_eval (le, h) (NewC v t)
+               (<[v:=LocV l]> le, <[l:=(t,IntV 0)]> h)
+  | GetEv le h v e l tl vl :
+      expr_eval le e (LocV l) →
+      h !! l = Some (tl, vl) →
+      cmd_eval (le, h) (GetC v e) (<[v:=vl]> le, h)
+  | SetEv le h lhs rhs l tl vr :
+      expr_eval le lhs (LocV l) →
+      (∃ vl, h !! l = Some (tl, vl)) →
+      expr_eval le rhs vr →
+      cmd_eval (le, h) (SetC lhs rhs) (le, <[l:=(tl,vr)]> h)
+  | SeqEv st1 st2 st3 fstc sndc :
+      cmd_eval st1 fstc st2 →
+      cmd_eval st2 sndc st3 →
+      cmd_eval st1 (SeqC fstc sndc) st3
+  | Cond1Ev st1 st2 cnd vc ifc elc :
+      expr_eval st1.1 cnd vc →
+      value_trueish vc →
+      cmd_eval st1 ifc st2 →
+      cmd_eval st1 (CondC cnd ifc elc) st2
+  | Cond2Ev st1 st2 cnd vc ifc elc :
+      expr_eval st1.1 cnd vc →
+      ¬value_trueish vc →
+      cmd_eval st1 elc st2 →
+      cmd_eval st1 (CondC cnd ifc elc) st2
+  | CondTag1Ev st1 st2 v t cmd :
+      tag_match st1 v t →
+      cmd_eval st1 cmd st2 →
+      cmd_eval st1 (CondTagC v t cmd) st2
+  | CondTag2Ev st v t cmd :
+      ¬tag_match st v t →
+      cmd_eval st (CondTagC v t cmd) st
+  | While1Ev st1 st2 st3 cnd vc cmd :
+      expr_eval st1.1 cnd vc →
+      value_trueish vc →
+      cmd_eval st1 cmd st2 →
+      cmd_eval st2 (WhileC cnd cmd) st3 →
+      cmd_eval st1 (WhileC cnd cmd) st3
+  | While2Ev st cnd vc cmd :
+      expr_eval st.1 cnd vc →
+      ¬value_trueish vc →
+      cmd_eval st (WhileC cnd cmd) st.
+
+Inductive prog_eval :
+    lang_prog → value → Prop :=
+  | ProgEv body le h ret val :
+      cmd_eval (∅,∅) body (le,h) →
+      expr_eval le ret val →
+      prog_eval (Prog body ret) val.
+
+Definition interp_local_tys
+    (lty : local_tys) (le : local_env) : iProp :=
+  (∀ v ty, ⌜lty !! v = Some ty⌝ -∗
+           ∃ val, ⌜le !! v = Some val⌝ ∗ interp_type ty val)%I.
+
+Lemma expr_adequacy e lty le ty val :
+  expr_eval le e val →
+  expr_has_ty lty e ty →
+  interp_local_tys lty le -∗
+  interp_type ty val.
+Proof.
+  (* the language is this simple that no
+     induction is necessary *)
+  case.
+  - move=> v val' ?. inversion_clear 1.
+    iIntros "#Hlty".
+    iDestruct ("Hlty" with "[//]") as (?) "[% H]".
+    simplify_eq. done.
+  - move=> lit. inversion_clear 1.
+    iIntros "_". rewrite interp_type_unfold /=.
+    rewrite /interp_int. by eauto.
+  - move=> op lhs rhs nl nr _ _.
+    inversion_clear 1.
+    iIntros "_". rewrite interp_type_unfold /=.
+    rewrite /interp_int. by eauto.
+Qed.
+
+Lemma interp_local_tys_update v lty le ty val :
+  interp_local_tys lty le -∗
+  interp_type ty val -∗
+  interp_local_tys (<[v:=ty]>lty) (<[v:=val]>le).
+Proof.
+  iIntros "#Hi #?". iIntros (v' ty') "H".
+  rewrite lookup_insert_Some.
+  iDestruct "H" as %[[<- <-]|[??]].
+  - iExists _. rewrite lookup_insert. by iSplit.
+  - rewrite lookup_insert_ne; last done. by iApply "Hi".
+Qed.
+
+Lemma heap_models_lookup l h tl vl t :
+  h !! l = Some (tl, vl) →
+  heap_models h -∗
+  interp_type (ClassT t) (LocV l) -∗
+  ∃ fty, heap_models h ∗
+         ⌜t = tl ∧ Δ !! t = Some fty⌝ ∗
+         ▷ interp_type fty vl.
+Proof.
+  move=>?. iIntros "Hh Hc".
+  rewrite interp_type_unfold /=.
+  iDestruct "Hc" as (??) "[H H◯]".
+  iDestruct "H" as %[[= <-]Hfty].
+  iDestruct "Hh" as (sh) "(H●&%&#Hh)".
+  iDestruct (own_valid_2 with "H● H◯") as "#Hv".
+  rewrite gmap_view_both_validI.
+  iDestruct "Hv" as "[_ HΦ]".
+  iDestruct ("Hh" with "[//]") as (?) "[H H▷]".
+  iRewrite "H" in "HΦ".
+  rewrite option_equivI prod_equivI /=.
+  iDestruct "HΦ" as "[-> HΦ]".
+  rewrite later_equivI.
+  iExists fty.
+  iSplitL. { iExists _. iFrame. by iSplit. }
+  iSplitR; first done.
+  iNext. rewrite discrete_fun_equivI.
+  iSpecialize ("HΦ" $! vl).
+  by iRewrite "HΦ" in "H▷".
+Qed.
+
+Lemma heap_models_update h l t v
+      (Φ : interpO) `{∀ v, Persistent (Φ v)} :
+  heap_models h -∗ (* ▷ *) Φ v -∗
+  sem_heap_mapsto l t Φ -∗
+  heap_models (<[l:=(t,v)]> h).
+Proof.
+  iIntros "Hh #HΦ #H◯".
+  iDestruct "Hh" as (sh) "(H●&%&#Hh)".
+  iDestruct (own_valid_2 with "H● H◯") as "#Hv".
+  rewrite gmap_view_both_validI.
+  iDestruct "Hv" as "[_ Hsh]".
+  iExists sh. iFrame.
+  iAssert ⌜is_Some (sh !! l)⌝%I as %?.
+  { move: (sh !! l) => [>|].
+    by iPureIntro; eauto.
+    by rewrite option_equivI;
+       iDestruct "Hsh" as "[]". }
+  iSplitR.
+  - iPureIntro.
+    rewrite dom_insert_lookup_L; first done.
+    apply (elem_of_dom (D:=gset loc)).
+    by rewrite -H0 elem_of_dom.
+  - iModIntro. iIntros (l' t' v') "H".
+    rewrite lookup_insert_Some.
+    iDestruct "H" as %[[<- [= <- <-]]|[??]].
+    + iExists Φ. by iSplit.
+    + by iApply "Hh".
+Qed.
+
+Notation "|=▷=>^ n Q" := (Nat.iter n (λ P, |==> ▷ P) Q)%I
+  (at level 99, n at level 9, Q at level 200,
+   format "|=▷=>^ n  Q") : bi_scope.
+
+Lemma updN_zero (Q : iProp) : (|=▷=>^0 Q) ⊣⊢ Q.
+Proof. done. Qed.
+
+Lemma updN_S n (Q : iProp) :
+  (|=▷=>^(S n) Q) ⊣⊢ |==> ▷ |=▷=>^n Q.
+Proof. done. Qed.
+
+Lemma updN_mono n (P Q : iProp) :
+  (P -∗ Q) → (|=▷=>^n P) -∗ (|=▷=>^n Q).
+Proof.
+  elim: n => [//|n HI H].
+  rewrite !updN_S.
+  iApply bupd_mono.
+  iApply bi.later_mono.
+  by iApply HI.
+Qed.
+
+(* (* We may want something like that to improve the
+      proof mode with the updN modality *)
+Global Instance into_wand_updN n p q (R P Q : iProp) :
+  IntoWand p q R P Q → IntoWand p q (|=▷=>^n R) (|=▷=>^n P) (|=▷=>^n Q).
+Proof.
+  rewrite /IntoWand /= => HR.
+  by rewrite !later_intuitionistically_if_2 -later_wand HR.
+Qed.
+Global Instance into_wand_later_args p q R P Q :
+  IntoWand p q R P Q → IntoWand' p q R (▷ P) (▷ Q).
+Proof.   rewrite /IntoWand' /IntoWand /= => HR. 
+           by rewrite !later_intuitionistically_if_2    
+         (later_intro (□?p R)) -later_wand HR.
+Qed.
+*)
+
+Lemma cmd_adequacy lty lty' st cmd st' :
+  cmd_eval st cmd st' →
+  cmd_has_ty lty cmd lty' →
+  ∃ n,
+    heap_models st.2 ∗ interp_local_tys lty st.1 -∗ |=▷=>^n
+    heap_models st'.2 ∗ interp_local_tys lty' st'.1.
+Proof.
+  move=> E. move: lty lty'. elim: E.
+  - move=>> ? /=. inversion_clear 1.
+    exists 0. iIntros "[? #Hle]".
+    rewrite updN_zero. iFrame.
+    iDestruct (expr_adequacy with "Hle")
+      as "#?"; try done.
+    by iApply interp_local_tys_update.
+  - move=>?? l v t ?? /=. inversion_clear 1.
+    (* we need one modality to update the
+       semantic heap *)
+    exists 1. iIntros "[Hh #Hle]".
+    rewrite updN_S updN_zero.
+    iDestruct "Hh" as (sh) "(H●&Hdom&#Hh)".
+    iDestruct "Hdom" as %Hdom.
+    iMod (own_update with "H●") as "[H● H◯]".
+    { apply (gmap_view_alloc _ l DfracDiscarded
+        (t, Next (interp_type IntT)));
+        last done.
+    apply (not_elem_of_dom (D:=gset loc)).
+    by rewrite Hdom not_elem_of_dom. }
+    iIntros "!> !>". iDestruct "H◯" as "#H◯".
+    iAssert (interp_type (ClassT t) (LocV l))
+      with "[]" as "#Hl".
+    { rewrite interp_type_unfold /=.
+      iExists _, _. by iSplit. }
+    iSplitL; last first.
+    by iApply interp_local_tys_update.
+    iExists _. iFrame. iSplit.
+    by rewrite !dom_insert_L Hdom.
+    iModIntro. iIntros (???) "Hlook".
+    rewrite lookup_insert_Some.
+    iDestruct "Hlook" as %[[<- [= <- <-]]|[Hℓ Hlook]].
+    + iExists _. rewrite lookup_insert.
+      iSplitR; first done.
+      rewrite (interp_type_unfold IntT) /=.
+      rewrite /interp_int. by eauto.
+    + rewrite lookup_insert_ne; last done.
+      by iApply "Hh".
+  - move=>> ?? /=. inversion_clear 1.
+    exists 1. iIntros "[Hh #Hle]".
+    iModIntro. (* keep the later *)
+    iDestruct (expr_adequacy with "Hle")
+      as "#He"; try done.
+    iDestruct (heap_models_lookup with "Hh He")
+      as (fty) "(Hh&Ht&Hv)"; first done.
+    rewrite H0. iDestruct "Ht" as %[?[=<-]].
+    rewrite bi.later_sep.
+    iSplitL "Hh"; first done.
+    iNext. by iApply interp_local_tys_update.
+  - move=>?? lhs rhs > ?[??]? /=.
+    inversion_clear 1. exists 0.
+    iIntros "[Hh #Hle]".
+    rewrite updN_zero. iSplitL; last done.
+    iDestruct (expr_adequacy lhs with "Hle")
+      as "#Hlhs"; try done.
+    iDestruct (expr_adequacy rhs with "Hle")
+      as "#Hrhs"; try done.
+    iDestruct (heap_models_lookup with "Hh Hlhs")
+      as (fty) "(Hh&Ht&?)"; first done.
+    rewrite H0. iDestruct "Ht" as %[[=<-][=<-]].
+    rewrite interp_type_unfold.
+    iDestruct "Hlhs" as (??) "(H&?)".
+    rewrite H0. iDestruct "H" as %[[=<-][=<-]].
+    iApply (heap_models_update with "Hh");
+      try done. by intros; apply _.
+  - move=>> ? Hfst ? Hsnd. inversion_clear 1.
+    apply Hfst in H0. apply Hsnd in H1.
+    clear Hfst Hsnd.
+    destruct H0 as [n1 Hfst].
+    destruct H1 as [n2 Hsnd].
+    exists (n1 + n2).
+    iIntros "H".
+    iDestruct (Hfst with "H") as "H".
+    iPoseProof (updN_mono with "H") as "H";
+      first done.
+    by rewrite Nat_iter_add.
+  - move=>> ?? ? Hifc ??. inversion_clear 1.
+    apply Hifc in H1. clear Hifc.
+    destruct H1 as [n Hifc]. exists n.
+    iIntros "H". iPoseProof (Hifc with "H") as "H".
+    done.
+  - move=>> ?? ? Helc ??. inversion_clear 1.
+    apply Helc in H2. clear Helc.
+    destruct H2 as [n Helc]. exists n.
+    iIntros "H". iPoseProof (Helc with "H") as "H".
+    done.
+  - move=>[le1 h1] ? v t ? [l /= [? [v' ?]]] ? H.
+    inversion_clear 1. apply H in H2. clear H.
+    destruct H2 as [n Hcmd]. exists n.
+    iIntros "H". iApply Hcmd. clear Hcmd n.
+    (* now for some fun :) *)
+    iDestruct "H" as "[Hh #Hlty]".
+    destruct H1 as [ty Hvty].
+    iDestruct ("Hlty" $! v with "[//]")
+      as (?) "[Hlev Hv]".
+    iDestruct "Hlev" as %Hlev.
+    rewrite -> Hlev in *. simplify_eq.
+    iDestruct (interp_type_loc_inversion with "Hv")
+      as (t') "Hv'".
+    iDestruct (heap_models_lookup with "Hh Hv'")
+      as (fty) "(Hh&Ht&_)"; first done.
+    iDestruct "Ht" as %[[=->]HΔ].
+    iFrame. (* not quite interp_local_tys_update *)
+    iIntros (??) "H". rewrite lookup_insert_Some.
+    iDestruct "H" as %[[<- <-]|[??]].
+    by iExists _; iSplit.
+    by iApply "Hlty".
+  - move=>> ?. inversion_clear 1.
+    by exists 0.
+  - (* this exactly the same thing as in the
+       sequence case *)
+    move=>> ??? Hitr_ ? Hcnt_. inversion 1; subst.
+    move: (Hitr_ _ _ H5) => [n1 Hitr]. clear Hitr_.
+    move: (Hcnt_ _ _ H) => [n2 Hcnt]. clear Hcnt_.
+    exists (n1 + n2).
+    iIntros "H".
+    iDestruct (Hitr with "H") as "H".
+    iPoseProof (updN_mono with "H") as "H";
+      first done.
+    by rewrite Nat_iter_add.
+  - move=>> ???. inversion_clear 1.
+    by exists 0.
 Qed.
 
 End proofs.
